updated FlatToRiscvDef

compiler/src/compiler/FlatToRiscvDef.v
@@ -514,10 +514,10 @@ Section FlatToRiscv1.
     Definition leak_Jal := ILeakage Jal_leakage.
     Definition leak_Jalr := ILeakage Jalr_leakage.
     
-    Definition bigtuple : Type := stmt Z * trace * list LeakageEvent * Z * word * Z * (trace -> list LeakageEvent -> list LeakageEvent * event).
+    Definition bigtuple : Type := stmt Z * trace * Z * word * Z * (trace -> list LeakageEvent -> list LeakageEvent * word).
   
     Definition project_tuple (tup : bigtuple) : nat * stmt Z :=
-      let '(s, k, rk_so_far, mypos, sp_val, stackoffset, f) := tup in
+      let '(s, k, mypos, sp_val, stackoffset, f) := tup in
       (length k, s).
 
     (* why take rk_so_far as an argument?
@@ -567,45 +567,47 @@ Section FlatToRiscv1.
     Print bigtuple.
     Definition rtransform_stmt_trace_body
       (tup : (*stmt Z * trace * trace * Z * word * Z * (trace -> trace -> list LeakageEvent * trace)*) bigtuple)
-      (rtransform_stmt_trace : forall othertup, lt_tuple othertup tup -> list LeakageEvent * event)
-      : list LeakageEvent * event.
+      (rtransform_stmt_trace : forall othertup, lt_tuple othertup tup -> list LeakageEvent * word)
+      : list LeakageEvent * word.
       refine (
           match tup as x return tup = x -> _ with
-          | (s, k, rk_so_far, mypos, sp_val, stackoffset, f) =>
+          | (s, k, mypos, sp_val, stackoffset, f) =>
               fun _ =>
               match s as x return s = x -> _ with
               | SLoad sz x y o =>
                   fun _ =>
                     match k with
                     | leak_word addr :: k' =>
-                        f [leak_word addr] (rk_so_far ++ [leak_load sz addr])
-                    | _ => (nil, leak_unit)
+                        f [leak_word addr] [leak_load sz addr]
+                    | _ => (nil, word.of_Z 0)
                     end
               | SStore sz x y o =>
                   fun _ =>
                     match k with
                     | leak_word addr :: k' =>
-                        f [leak_word addr] (rk_so_far ++ [leak_store sz addr])
-                    | _ => (nil, leak_unit)
+                        f [leak_word addr] [leak_store sz addr]
+                    | _ => (nil, word.of_Z 0)
                     end
               | SInlinetable sz x t i =>
                   fun _ =>
                     match k with
                     | leak_word i' :: k' =>
-                        f [leak_word i'] (rk_so_far ++ [leak_Jal; leak_Add; leak_load sz (word.add (word.add (word.add program_base (word.of_Z mypos)) (word.of_Z 4)) i')])
-                    | _ => (nil, leak_unit)
+                        f [leak_word i'] [leak_Jal; leak_Add; leak_load sz (word.add (word.add (word.add program_base (word.of_Z mypos)) (word.of_Z 4)) i')]
+                    | _ => (nil, word.of_Z 0)
                     end
               | SStackalloc _ n body =>
                   fun _ =>
                     match k as x return k = x -> _ with
-                    | consume_word addr :: k' =>
+                    | leak_unit :: k' =>
                         fun _ =>
-                          rtransform_stmt_trace (body, k', rk_so_far ++ [ leak_Addi ], mypos + 4, sp_val, stackoffset - n, fun skip => f (consume_word addr :: skip)) _
-                    | _ => fun _ => (nil, consume_word (word.add sp_val (word.of_Z (stackoffset - n))))
+                          let before := [leak_unit] in
+                          let rbefore := [leak_Addi] in
+                          rtransform_stmt_trace (body, k', mypos + 4, sp_val, stackoffset - n, fun skip rk => f (before ++ skip) (rbefore ++ rk)) _
+                    | _ => fun _ => (nil, word.add sp_val (word.of_Z (stackoffset - n)))
                     end eq_refl
               | SLit _ v =>
                   fun _ =>
-                    f [] (rk_so_far ++ leak_lit v)
+                    f [] (leak_lit v)
               | SOp _ op _ operand2 =>
                   fun _ =>
                     let newt_operands :=
@@ -630,66 +632,67 @@ Section FlatToRiscv1.
                     | Some (newt, x1, x2) =>
                         match leak_op op operand2 x1 x2 with
                         | Some l =>
-                            f newt (rk_so_far ++ l)
-                        | None => (nil, leak_unit)
+                            f newt l
+                        | None => (nil, word.of_Z 0)
                         end
-                    | None => (nil, leak_unit)
+                    | None => (nil, word.of_Z 0)
                     end
               | SSet _ _ =>
                   fun _ =>
-                    f [] (rk_so_far ++ [ leak_Add ])
+                    f [] [ leak_Add ]
               | SIf cond bThen bElse =>
                   fun _ =>
                     let thenLength := Z.of_nat (length (compile_stmt (mypos + 4) stackoffset bThen)) in
                     match k as x return k = x -> _ with
                     | leak_bool b :: k' =>
                         fun _ =>
+                          let before := [leak_bool b] in
+                          let rbefore := [ leak_bcond_by_inverting cond (negb b) ] in
                           rtransform_stmt_trace (if b then bThen else bElse,
                               k',
-                              rk_so_far ++ [ leak_bcond_by_inverting cond (negb b) ],
                               if b then mypos + 4 else mypos + 4 + 4 * thenLength + 4,
                               sp_val,
                               stackoffset,
-                              fun skip rk_so_far' =>
-                                f (leak_bool b :: skip)
-                                  (rk_so_far' ++ if b then [leak_Jal] else [])) _
-                    | _ => fun _ => (nil, leak_unit)
+                              fun skip rk =>
+                                f (before ++ skip)
+                                  (rbefore ++ rk ++ if b then [leak_Jal] else [])) _
+                    | _ => fun _ => (nil, word.of_Z 0)
                     end eq_refl
               | SLoop body1 cond body2 =>
                   fun _ =>
                     let body1Length := Z.of_nat (length (compile_stmt mypos stackoffset body1)) in
-                    rtransform_stmt_trace (body1, k, rk_so_far, mypos, sp_val, stackoffset,
-                        fun skip rk_so_far'  =>
+                    rtransform_stmt_trace (body1, k, mypos, sp_val, stackoffset,
+                        fun skip rk  =>
                           Let_In_pf_nd (List.skipn (length skip) k)
                           (fun k' _ =>
                              match k' as x return k' = x -> _ with
                              | leak_bool true :: k'' =>
                                  fun _ =>
+                                   let rbefore1 := [ leak_bcond_by_inverting cond (negb true) ] in
                                    rtransform_stmt_trace (body2,
                                        k'',
-                                       rk_so_far' ++ [ leak_bcond_by_inverting cond (negb true) ],
                                        mypos + (body1Length + 1) * 4, sp_val, stackoffset,
-                                       fun skip' rk_so_far'' =>
+                                       fun skip' rk' =>
                                          let k''' := List.skipn (length skip') k'' in
+                                         let rbefore2 := [leak_Jal] in
                                          rtransform_stmt_trace (s,
                                              k''',
-                                             rk_so_far'' ++ [ leak_Jal ],
                                              mypos, sp_val, stackoffset,
-                                             fun skip'' => f (skip ++ leak_bool true :: skip' ++ skip'')) _) _
+                                             fun skip'' rk'' => f (skip ++ leak_bool true :: skip' ++ skip'') (rk ++ rbefore1 ++ rk' ++ rbefore2 ++ rk'')) _) _
                              | leak_bool false :: k'' =>
                                  fun _ =>
-                                   f (skip ++ [leak_bool false]) (rk_so_far' ++ [ leak_bcond_by_inverting cond (negb false) ])
-                             | _ => fun _ => (nil, leak_unit)
+                                   f (skip ++ [leak_bool false]) (rk ++ [ leak_bcond_by_inverting cond (negb false) ])
+                             | _ => fun _ => (nil, word.of_Z 0)
                              end eq_refl)) _
               | SSeq s1 s2 =>
                   fun _ =>
                     let s1Length := Z.of_nat (length (compile_stmt mypos stackoffset s1)) in
-                    rtransform_stmt_trace (s1, k, rk_so_far, mypos, sp_val, stackoffset,
-                        fun skip rk_so_far' =>
+                    rtransform_stmt_trace (s1, k, mypos, sp_val, stackoffset,
+                        fun skip rk =>
                           let k' := List.skipn (length skip) k in
-                          rtransform_stmt_trace (s2, k', rk_so_far', mypos + 4 * s1Length, sp_val, stackoffset,
-                              fun skip' => f (skip ++ skip')) _) _
-              | SSkip => fun _ => f [] rk_so_far
+                          rtransform_stmt_trace (s2, k', mypos + 4 * s1Length, sp_val, stackoffset,
+                              fun skip' rk' => f (skip ++ skip') (rk ++ rk')) _) _
+              | SSkip => fun _ => f [] []
               | SCall resvars fname argvars =>
                   fun _ =>
                     match k as x return k = x -> _ with
@@ -698,23 +701,23 @@ Section FlatToRiscv1.
                           match map.get e_env fname, map.get e fname with
                           | Some (params, rets, fbody), Some fpos =>
                               let '(beforeBody, afterBody, mypos', sp_val', stackoffset') := rtransform_fun_trace_helper fpos sp_val rets fbody in
+                              let rbefore := leak_Jal (* jump to compiled function *) :: beforeBody in
                               rtransform_stmt_trace (fbody,
                                   k',
-                                  rk_so_far ++ leak_Jal (* jump to compiled function *) :: beforeBody,
                                   mypos', sp_val', stackoffset',
-                                  fun skip rk_so_far' =>
+                                  fun skip rk =>
                                     let k'' := List.skipn (length skip) k' in
-                                    f (leak_unit :: skip) (rk_so_far' ++ afterBody)) _
-                          | _, _ => (nil, leak_unit)
+                                    f (leak_unit :: skip) (rbefore ++ rk ++ afterBody)) _
+                          | _, _ => (nil, word.of_Z 0)
                           end
-                    | _ => fun _ => (nil, leak_unit)
+                    | _ => fun _ => (nil, word.of_Z 0)
                     end eq_refl
               | SInteract _ _ _ =>
                   fun _ =>
                     match k with
                     | leak_list l :: k' =>
-                        f [leak_list l] (rk_so_far ++ leak_ext_call e mypos stackoffset s l)
-                    | _ => (nil, leak_unit)
+                        f [leak_list l] (leak_ext_call e mypos stackoffset s l)
+                    | _ => (nil, word.of_Z 0)
                     end
               end eq_refl
           end eq_refl).
@@ -741,11 +744,12 @@ Section FlatToRiscv1.
 
       Definition rtransform_stmt_trace
         := my_Fix _ _ lt_tuple_wf _ rtransform_stmt_trace_body.
-      
+
+      Print bigtuple.
       Definition Equiv (x y : bigtuple) :=
-        let '(x1, x2, x3, x4, x5, x6, fx) := x in
-        let '(y1, y2, y3, y4, y5, y6, fy) := y in
-        (x1, x2, x3, x4, x5, x6) = (y1, y2, y3, y4, y5, y6) /\
+        let '(x1, x2, x3, x4, x5, fx) := x in
+        let '(y1, y2, y3, y4, y5, fy) := y in
+        (x1, x2, x3, x4, x5) = (y1, y2, y3, y4, y5) /\
           forall k rk,
             fx k rk = fy k rk.
 
@@ -753,8 +757,8 @@ Section FlatToRiscv1.
         Equiv x y -> Equiv y x.
       Proof.
         intros. cbv [Equiv] in *.
-        destruct x as [ [ [ [ [ [x1 x2] x3] x4] x5] x6] fx].
-        destruct y as [ [ [ [ [ [y1 y2] y3] y4] y5] y6] fy].
+        destruct x as [ [ [ [ [x1 x2] x3] x4] x5] fx].
+        destruct y as [ [ [ [ [y1 y2] y3] y4] y5] fy].
         destruct H as [H1 H2]. auto.
       Qed.
 
@@ -762,9 +766,9 @@ Section FlatToRiscv1.
         Equiv x1 x2 -> lt_tuple x1 y -> lt_tuple x2 y.
       Proof.
         cbv [lt_tuple Equiv]. 
-        destruct x1 as [ [ [ [ [ [x1_1 x2_1] x3_1] x4_1] x5_1] x6_1] fx_1].
-        destruct x2 as [ [ [ [ [ [x1_2 x2_2] x3_2] x4_2] x5_2] x6_2] fx_2].
-        destruct y as [ [ [ [ [ [y1 y2] y3] y4] y5] y6] fy].
+        destruct x1 as [ [ [ [ [x1_1 x2_1] x3_1] x4_1] x5_1] fx_1].
+        destruct x2 as [ [ [ [ [x1_2 x2_2] x3_2] x4_2] x5_2] fx_2].
+        destruct y as [ [ [ [ [y1 y2] y3] y4] y5] fy].
         cbn [project_tuple].
         intros [H1 H2] H3. injection H1. intros. subst. assumption.
       Qed.
@@ -776,15 +780,15 @@ Section FlatToRiscv1.
       Proof. intros. subst. reflexivity. Qed.        
 
       Lemma rtransform_stmt_trace_body_ext :
-        forall (x1 x2 : bigtuple) (f1 : forall y : bigtuple, lt_tuple y x1 -> list LeakageEvent * event)
-               (f2 : forall y : bigtuple, lt_tuple y x2 -> list LeakageEvent * event),
+        forall (x1 x2 : bigtuple) (f1 : forall y : bigtuple, lt_tuple y x1 -> list LeakageEvent * word)
+               (f2 : forall y : bigtuple, lt_tuple y x2 -> list LeakageEvent * word),
           Equiv x1 x2 ->
           (forall (y1 y2 : bigtuple) (p1 : lt_tuple y1 x1) (p2 : lt_tuple y2 x2),
               Equiv y1 y2 -> f1 y1 p1 = f2 y2 p2) -> @rtransform_stmt_trace_body x1 f1 = @rtransform_stmt_trace_body x2 f2.
       Proof.
         intros. cbv [rtransform_stmt_trace_body]. cbv beta.
-        destruct x1 as [ [ [ [ [ [s_1 k_1] rk_so_far_1] mypos_1] sp_val_1] stackoffset_1] f_1].
-        destruct x2 as [ [ [ [ [ [s_2 k_2] rk_so_far_2] mypos_2] sp_val_2] stackoffset_2] f_2].
+        destruct x1 as [ [ [ [ [s_1 k_1] mypos_1] sp_val_1] stackoffset_1] f_1].
+        destruct x2 as [ [ [ [ [s_2 k_2] mypos_2] sp_val_2] stackoffset_2] f_2].
         cbv [Equiv] in H. destruct H as [H1 H2]. injection H1. intros. subst. clear H1.
         repeat (Tactics.destruct_one_match || reflexivity || apply app_eq || apply H3 || intros || apply H0 || cbv [Equiv]; intuition).
         all: try apply Let_In_pf_nd_ext; intros.
@@ -803,7 +807,7 @@ Section FlatToRiscv1.
         cbv [rtransform_stmt_trace]. Check my_Fix_eq.
         apply my_Fix_eq with (E1:=Equiv) (x1:=tup) (x2:=tup).
         { apply rtransform_stmt_trace_body_ext. }
-        { cbv [Equiv]. destruct tup as [ [ [ [ [ [x1 x2] x3] x4] x5] x6] fx]. auto. }
+        { cbv [Equiv]. destruct tup as [ [ [ [ [x1 x2] x3] x4] x5] fx]. auto. }
       Qed.
 
       Lemma rtransform_stmt_trace_ext :
@@ -819,12 +823,12 @@ Section FlatToRiscv1.
       Qed.
       
       Definition rtransform_fun_trace 
-        (k : trace) (rk_so_far : list LeakageEvent) (fpos : Z) (sp_val : word)
+        (k : trace) (fpos : Z) (sp_val : word)
         (rets : list Z) fbody
-        (f : trace -> list LeakageEvent -> list LeakageEvent * event) :=
+        (f : trace -> list LeakageEvent -> list LeakageEvent * word) :=
         let '(beforeBody, afterBody, mypos', sp_val', stackoffset') := rtransform_fun_trace_helper fpos sp_val rets fbody in
-        rtransform_stmt_trace (fbody, k, rk_so_far ++ beforeBody, mypos', sp_val', stackoffset',
-            fun skip rk_so_far' => f skip (rk_so_far' ++ afterBody)).
+        rtransform_stmt_trace (fbody, k, mypos', sp_val', stackoffset',
+            fun skip rk => f skip (beforeBody ++ rk ++ afterBody)).
     End WithOtherEnv.
   End WithEnv.
 
